proof/invariant-abstract/ARM/ArchCSpace_AI.thy
@@ -23,7 +23,7 @@ named_theorems CSpace_AI_assms
 (* FIXME: move? *)
 lemma getActiveIRQ_wp [CSpace_AI_assms]:
   "irq_state_independent_A P \<Longrightarrow>
-   valid P (do_machine_op getActiveIRQ) (\<lambda>_. P)"
+   valid P (do_machine_op (getActiveIRQ in_kernel)) (\<lambda>_. P)"
   apply (simp add: getActiveIRQ_def do_machine_op_def split_def exec_gets
                    select_f_select[simplified liftM_def]
                    select_modify_comm gets_machine_state_modify)
@@ -98,8 +98,8 @@ lemma set_free_index_invs [CSpace_AI_assms]:
   apply (simp add:valid_irq_node_def)
   apply wps
  
-  apply (wp hoare_vcg_all_lift set_cap_irq_handlers set_cap_arch_objs set_cap_valid_arch_caps
-    set_cap_valid_global_objs set_cap_irq_handlers cap_table_at_lift_valid set_cap_typ_at
+  apply (wp hoare_vcg_all_lift set_cap_irq_handlers set_cap_vspace_objs set_cap_valid_arch_caps
+    set_cap_irq_handlers cap_table_at_lift_valid set_cap_typ_at
     set_cap_cap_refs_respects_device_region_spec[where ptr = cref])
   apply (clarsimp simp:cte_wp_at_caps_of_state)
   apply (rule conjI,simp add:valid_pspace_def)
