proof/invariant-abstract/ARM/ArchRetype_AI.thy
@@ -57,6 +57,7 @@ lemma retype_region_ret_folded [Retype_AI_assms]:
   done
 
 declare store_pde_state_refs_of [wp]
+declare store_pde_state_hyp_refs_of [wp]
 
 (* These also prove facts about copy_global_mappings *)
 crunch pspace_aligned[wp]: init_arch_objects "pspace_aligned"
@@ -82,7 +83,7 @@ lemma mdb_cte_at_store_pde[wp]:
 done
 
 lemma get_pde_valid[wp]:
-  "\<lbrace>valid_arch_objs 
+  "\<lbrace>valid_vspace_objs
     and \<exists>\<rhd> (x && ~~mask pd_bits) 
     and K (ucast (x && mask pd_bits >> 2) \<notin> kernel_mapping_slots)\<rbrace> 
    get_pde x 
@@ -90,12 +91,12 @@ lemma get_pde_valid[wp]:
   apply (simp add: get_pde_def)
   apply wp
   apply clarsimp
-  apply (drule (2) valid_arch_objsD)
+  apply (drule (2) valid_vspace_objsD)
   apply simp
   done
 
 lemma get_master_pde_valid[wp]:
-  "\<lbrace>valid_arch_objs
+  "\<lbrace>valid_vspace_objs
     and \<exists>\<rhd> (x && ~~mask pd_bits)
     and K (ucast (x && mask pd_bits >> 2) \<notin> kernel_mapping_slots)\<rbrace>
    get_master_pde x
@@ -106,7 +107,7 @@ lemma get_master_pde_valid[wp]:
      apply (clarsimp simp: mask_lower_twice pd_bits_def pageBits_def)+
   apply (drule sym)
   apply (drule (1) ko_at_obj_congD, clarsimp)
-  apply (drule (2) valid_arch_objsD)
+  apply (drule (2) valid_vspace_objsD)
   apply simp
   apply (erule notE, erule bspec)
   apply (clarsimp simp: kernel_mapping_slots_def not_le)
@@ -157,6 +158,9 @@ crunch zombies[wp]: copy_global_mappings "zombies_final"
   (wp: crunch_wps)
 
 crunch state_refs_of[wp]: copy_global_mappings "\<lambda>s. P (state_refs_of s)"
+  (wp: crunch_wps)
+
+crunch state_hyp_refs_of[wp]: copy_global_mappings "\<lambda>s. P (state_hyp_refs_of s)"
   (wp: crunch_wps)
 
 crunch valid_idle[wp]: copy_global_mappings "valid_idle"
@@ -235,7 +239,7 @@ lemma glob_vs_refs_add_one':
 
 
 lemma store_pde_map_global_valid_arch_caps:
-  "\<lbrace>valid_arch_caps and valid_objs and valid_arch_objs
+  "\<lbrace>valid_arch_caps and valid_objs and valid_vspace_objs
      and valid_arch_state and valid_global_objs
      and K (valid_pde_mappings pde)
      and K (VSRef (p && mask pd_bits >> 2) (Some APageDirectory)
@@ -255,7 +259,7 @@ lemma store_pde_map_global_valid_arch_caps:
       apply (rule arg_cong[where f=Ex], rule ext, fastforce)
      apply clarsimp
      apply (rule conjI, clarsimp)
-     apply (drule valid_arch_objsD, simp add: obj_at_def, simp+)[1]
+     apply (drule valid_vspace_objsD, simp add: obj_at_def, simp+)[1]
     apply (rule impI, rule disjI2)
     apply (simp add: empty_table_def)
    apply clarsimp
@@ -284,18 +288,18 @@ lemma store_pde_map_global_valid_arch_caps:
   done
 
 
-lemma store_pde_map_global_valid_arch_objs:
-  "\<lbrace>valid_arch_objs and valid_arch_state and valid_global_objs
+lemma store_pde_map_global_valid_vspace_objs:
+  "\<lbrace>valid_vspace_objs and valid_arch_state and valid_global_objs
         and K (VSRef (p && mask pd_bits >> 2) (Some APageDirectory) \<in> kernel_vsrefs)\<rbrace>
     store_pde p pde
-   \<lbrace>\<lambda>rv. valid_arch_objs\<rbrace>"
+   \<lbrace>\<lambda>rv. valid_vspace_objs\<rbrace>"
   apply (simp add: store_pde_def)
-  apply (wp set_pd_arch_objs_map[where T="{}" and S="{}"])
+  apply (wp set_pd_vspace_objs_map[where T="{}" and S="{}"])
   apply (clarsimp simp: obj_at_def kernel_vsrefs_kernel_mapping_slots[symmetric])
   apply (intro conjI)
    apply (erule vs_refs_add_one'')
   apply clarsimp
-  apply (drule valid_arch_objsD, simp add: obj_at_def, simp+)
+  apply (drule valid_vspace_objsD, simp add: obj_at_def, simp+)
   apply clarsimp
   done
 
@@ -465,7 +469,7 @@ lemma copy_global_invs_mappings_restricted:
    apply (rule hoare_pre)
     apply (wp valid_irq_node_typ valid_irq_handlers_lift
               store_pde_map_global_valid_arch_caps
-              store_pde_map_global_valid_arch_objs
+              store_pde_map_global_valid_vspace_objs
               store_pde_valid_kernel_mappings_map_global
               get_pde_wp)
    apply (clarsimp simp: valid_global_objs_def)
@@ -709,6 +713,11 @@ lemma valid_untyped_helper [Retype_AI_assms]:
   apply blast (* set arith  *)
   done
   qed
+
+lemma valid_default_arch_tcb:
+  "\<And>s. valid_arch_tcb default_arch_tcb s"
+  by (simp add: default_arch_tcb_def valid_arch_tcb_def)
+
 end
 
 
@@ -810,6 +819,17 @@ lemma vs_lookup_pages':
   apply simp
   done
 
+lemma hyp_refs_eq:
+  "ARM.state_hyp_refs_of s' = ARM.state_hyp_refs_of s"
+  unfolding s'_def ps_def
+  apply (clarsimp intro!: ext simp: state_hyp_refs_of_def
+                    simp: orthr
+                   split: option.splits)
+  apply (cases ty, simp_all add: tyunt default_object_def default_tcb_def
+                                 hyp_refs_of_def tcb_hyp_refs_def
+                                 default_arch_tcb_def)
+  done
+
 end
 
 
@@ -817,7 +837,13 @@ context retype_region_proofs_arch begin
 
 lemma valid_arch_obj_pres:
   "valid_arch_obj ao s \<Longrightarrow> valid_arch_obj ao s'"
-  apply (cases ao; simp add: obj_at_pres)
+  apply (cases ao; simp add: valid_arch_obj_def obj_at_pres)
+     apply (erule allEI ballEI; rename_tac t i; case_tac "t i"; fastforce simp: data_at_def obj_at_pres)+
+  done
+
+lemma valid_vspace_obj_pres:
+  "valid_vspace_obj ao s \<Longrightarrow> valid_vspace_obj ao s'"
+  apply (cases ao; simp add: valid_vspace_obj_def obj_at_pres)
      apply (erule allEI ballEI; rename_tac t i; case_tac "t i"; fastforce simp: data_at_def obj_at_pres)+
   done
 
@@ -827,9 +853,35 @@ end
 context retype_region_proofs begin
 
 interpretation retype_region_proofs_arch ..
+thm valid_arch_objsI
+lemma valid_vspace_objs':
+  assumes va: "valid_vspace_objs s"
+  shows "valid_vspace_objs s'"
+proof
+  fix p ao
+  assume p: "(\<exists>\<rhd> p) s'"
+  assume "ko_at (ArchObj ao) p s'"
+  hence "ko_at (ArchObj ao) p s \<or> ArchObj ao = default_object ty dev us"
+    by (simp add: ps_def obj_at_def s'_def split: if_split_asm)
+  moreover
+  { assume "ArchObj ao = default_object ty dev us" with tyunt
+    have "valid_vspace_obj ao s'" by (rule valid_vspace_obj_default)
+  }
+  moreover
+  { assume "ko_at (ArchObj ao) p s"
+    with va p
+    have "valid_vspace_obj ao s"
+      by (auto simp: vs_lookup' elim: valid_vspace_objsD)
+    hence "valid_vspace_obj ao s'"
+      by (rule valid_vspace_obj_pres)
+  }
+  ultimately
+  show "valid_vspace_obj ao s'" by blast
+qed
+
 
 lemma valid_arch_objs':
-  assumes va: "valid_arch_objs s" 
+  assumes va: "valid_arch_objs s"
   shows "valid_arch_objs s'"
 proof
   fix p ao
@@ -854,7 +906,10 @@ proof
 qed
 
 (* ML \<open>val pre_ctxt_0 = @{context}\<close> *)
-sublocale retype_region_proofs_gen?: retype_region_proofs_gen ..
+sublocale retype_region_proofs_gen?: retype_region_proofs_gen
+ by (unfold_locales,
+        auto simp: hyp_refs_eq[simplified s'_def ps_def]
+                  valid_default_arch_tcb)
 (* local_setup \<open>note_new_facts pre_ctxt_0\<close> *)
 
 end
@@ -1018,10 +1073,10 @@ lemma valid_arch_caps:
 
 lemma valid_global_objs:
   "valid_global_objs s \<Longrightarrow> valid_global_objs s'"
-  apply (simp add: valid_global_objs_def valid_ao_at_def)
+  apply (simp add: valid_global_objs_def valid_vso_at_def)
   apply (elim conjE, intro conjI ballI)
     apply (erule exEI)
-    apply (simp add: obj_at_pres valid_arch_obj_pres)
+    apply (simp add: obj_at_pres valid_vspace_obj_pres)
    apply (simp add: obj_at_pres)
   apply (rule exEI, erule(1) bspec)
   apply (simp add: obj_at_pres valid_arch_obj_pres)
@@ -1174,7 +1229,7 @@ lemma post_retype_invs:
                      valid_global_refs valid_arch_state
                      valid_irq_node_def obj_at_pres
                      valid_arch_caps valid_global_objs
-                     valid_arch_objs' valid_irq_handlers
+                     valid_vspace_objs' valid_irq_handlers
                      valid_mdb_rep2 mdb_and_revokable
                      valid_pspace cur_tcb only_idle
                      valid_kernel_mappings valid_asid_map
@@ -1190,7 +1245,7 @@ sublocale retype_region_proofs_invs?: retype_region_proofs_invs
   where region_in_kernel_window = region_in_kernel_window
     and post_retype_invs_check = post_retype_invs_check
     and post_retype_invs = post_retype_invs
-  using post_retype_invs valid_cap valid_global_refs valid_arch_state valid_arch_objs'
+  using post_retype_invs valid_cap valid_global_refs valid_arch_state valid_vspace_objs'
   by unfold_locales (auto simp: s'_def ps_def)
 
 (* local_setup \<open>note_new_facts pre_ctxt_1\<close> *)
